Rewrote local variable theory, so that now we have store mapping names to values. This works much better than previous attempts, since checking independence (etc.) can use the name strings.

UTP/ITree_Local_Var.thy
@@ -225,171 +225,161 @@ qed
 
 subsection \<open> Local Variable Stack \<close>
 
+type_synonym uname = "String.literal"
+
+text \<open> We model the store as a finite partial function from names (strings) to values in the 
+  universe defined above. \<close>
+
 zstore lvar =
-  lstack :: "uval list"
+  lstore :: "uname \<Zffun> uval"
 
-text \<open> Extend the variable stack \<close>
+subsection \<open> Identifiers as Strings \<close>
 
-definition open_var :: "utype \<Rightarrow> ('e, 'a lvar_scheme) htree" where
-"open_var a = (lstack := lstack @ [uval_default \<guillemotleft>a\<guillemotright>])"
+text \<open> Each local variable is assigned the same name as the Isabelle identifier used to introduce
+  the name in the binder. For this reason, we need to convert identifiers into strings. \<close>
 
-text \<open> Reduce the variable stack \<close>
+syntax
+  "_id_string"     :: "id \<Rightarrow> string" ("IDSTR'(_')")
+  "_id_literal"    :: "id \<Rightarrow> String.literal" ("IDLIT'(_')")
 
-definition close_var :: "('e, 'a lvar_scheme) htree" where
-"close_var = (lstack := butlast lstack)"
+parse_translation \<open>
+let
+  fun id_string_tr [Free (full_name, _)] = HOLogic.mk_string full_name
+    | id_string_tr [Const (full_name, _)] = HOLogic.mk_string full_name
+    | id_string_tr _ = raise Match;
+  fun id_literal_tr [Free (full_name, _)] = HOLogic.mk_literal full_name
+    | id_literal_tr [Const (full_name, _)] = HOLogic.mk_literal full_name
+    | id_literal_tr _ = raise Match;
 
-text \<open> A lens pointing to one of the locations in the stack. The first parameter denotes the
-  number of variables blocks that were opened within the block for this particular variable
-  (like a de-Bruijn index) \<close>
+in
+  [(@{syntax_const "_id_string"}, K id_string_tr)
+  ,(@{syntax_const "_id_literal"}, K id_literal_tr)]
+end
+\<close>
 
-definition lvar_lens :: "nat \<Rightarrow> ('v::injval \<Longrightarrow> 's lvar_scheme)" where 
-"lvar_lens n = (uval_lens ;\<^sub>L list_lens n ;\<^sub>L lstack)"
+subsection \<open> Local Variable Lenses \<close>
+
+text \<open> The local variable lens projects the store, followed by the value (@{typ uval}) at the given 
+  name, followed by projecting out a value of the correct type. \<close>
+
+definition lvar_lens :: "uname \<Rightarrow> ('a::injval \<Longrightarrow> 's lvar_scheme)" where 
+"lvar_lens n = (uval_lens ;\<^sub>L ffun_lens n ;\<^sub>L lstore)" 
 
 lemma mwb_lvar_lens [simp]: "mwb_lens (lvar_lens n)"
-  by (simp add: lvar_lens_def list_mwb_lens comp_mwb_lens)
+  by (simp add: comp_mwb_lens lvar_lens_def)
 
-lemma source_lvar_lens: 
-  "\<S>\<^bsub>lvar_lens n s :: 'b \<Longrightarrow> _\<^esub> 
-   = {s'. length (get\<^bsub>lstack\<^esub> s) - Suc n < length (get\<^bsub>lstack\<^esub> s')
-        \<and> get\<^bsub>lstack\<^esub> s' ! (length (get\<^bsub>lstack\<^esub> s) - Suc n) \<in> uvals (utyp TYPE('b::injval))}"
-  apply (simp add: lvar_lens_def lens_defined_def comp_mwb_lens list_mwb_lens source_lens_comp source_list_lens source_uval_lens univ_var_def id_lens_def)
-  apply (simp add: list_lens_def nth'_def)
-  apply auto
-  apply (metis UNIV_I lstack_vwb_lens vwb_lens_iff_mwb_UNIV_src)
-  done
+lemma pfun_lens_indep: "x \<noteq> y \<Longrightarrow> ffun_lens x \<bowtie> ffun_lens y"
+  by (unfold_locales, simp_all add: ffun_lens_def ffun_upd_comm)
 
-definition lv_lens :: "('v::injval \<Longrightarrow> 's lvar_scheme) \<Rightarrow> nat \<Rightarrow> bool" where
-"lv_lens x i = (x = uval_lens ;\<^sub>L list_lens i ;\<^sub>L lstack)"
+lemma lvar_lens_indep [simp]: "m \<noteq> n \<Longrightarrow> lvar_lens m \<bowtie> lvar_lens n"
+  by (simp add: lvar_lens_def pfun_lens_indep lens_indep_left_ext lens_indep_right_ext)
 
-lemma lv_lens_then_mwb: "lv_lens x i \<Longrightarrow> mwb_lens x"
-  by (auto simp add: lv_lens_def comp_mwb_lens list_mwb_lens)
-
-lemma lv_lens_indep [simp]: "\<lbrakk> i \<noteq> j; lv_lens x i; lv_lens y j \<rbrakk> \<Longrightarrow> x \<bowtie> y"
-  by (simp add: lv_lens_def lens_indep_left_ext lens_indep_right_ext list_lens_indep)
-
-text \<open> The next predicate characterises the location of a local variable in the stack. \<close>
-
-definition lv_at :: "('v::injval \<Longrightarrow> 's lvar_scheme) \<Rightarrow> nat \<Rightarrow> 's lvar_scheme \<Rightarrow> bool" where 
-  "lv_at x n = (\<lambda> s. 
-                 \<comment> \<open> The stack is big enough \<close>
-                 length (get\<^bsub>lstack\<^esub> s) > n 
-                 \<comment> \<open> The value at the location has the correct type \<close>
-               \<and> uval_type (get\<^bsub>lstack\<^esub> s ! n) = Some (utyp TYPE('v))
-                 \<comment> \<open> The lens is defined as a local variable lens \<close> 
-               \<and> x = lvar_lens n)"
-
-lemma lv_at_indep_out_stack1 [simp]: "\<lbrakk> lv_at x n s; lstack \<bowtie> y \<rbrakk> \<Longrightarrow> x \<bowtie> y"
-  by (simp add: lens_indep_left_ext lv_at_def lvar_lens_def) 
-
-lemma lv_at_indep_out_stack2 [simp]: "\<lbrakk> lv_at x n s; lstack \<bowtie> y \<rbrakk> \<Longrightarrow> y \<bowtie> x"
-  by (metis lens_indep_right_ext lens_indep_sym lv_at_def lvar_lens_def)
-
-lemma lv_at_indep_in_stack [simp]: "\<lbrakk> lv_at x m s; lv_at y n s; m \<noteq> n \<rbrakk> \<Longrightarrow> x \<bowtie> y"
-  by (simp add: lv_at_def lvar_lens_def lens_comp_indep_cong)
-     (metis Suc_diff_Suc diff_less_mono2 lens_indep_left_ext lens_indep_right_ext list_lens_indep nat_neq_iff)
-
-lemma lv_at_grow_stack_1 [usubst]: "(lv_at x n)\<lbrakk>butlast lstack/lstack\<rbrakk> = lv_at x n"
-  apply (auto simp add: lv_at_def lvar_lens_def subst_app_def subst_upd_def fun_eq_iff nth_butlast)
-  oops
-  
-lemma lv_at_grow_stack_2 [simp]: "lv_at x n ([lstack \<leadsto> butlast ($lstack)] s) = lv_at x (n + 1) s"
-  apply (auto simp add: lv_at_def lvar_lens_def subst_app_def subst_upd_def fun_eq_iff nth_butlast)
-  oops
-
-lemma lv_at_mwb: "lv_at x n s \<Longrightarrow> mwb_lens x"
-  by (metis comp_mwb_lens list_mwb_lens lstack_vwb_lens lv_at_def lvar_lens_def mwb_uval_lens vwb_lens_mwb)
+lemma get_ffun_lens: "get\<^bsub>ffun_lens i\<^esub> s = s(i)\<^sub>f"
+  by (simp add: ffun_lens_def)
 
 lemma vwb_src_UNIV [simp]: "vwb_lens X \<Longrightarrow> \<S>\<^bsub>X\<^esub> = UNIV"
   by (meson vwb_lens_iff_mwb_UNIV_src)
 
-lemma lv_at_then_defined [simp]: "lv_at x n s \<Longrightarrow> \<^bold>D(x) s"
-  apply (auto simp add: lv_at_def lvar_lens_def lens_defined_def comp_mwb_lens list_mwb_lens source_lens_comp source_list_lens source_uval_lens univ_var_def id_lens_def)
-  apply (auto simp add: list_lens_def nth'_def uvals_def)
-  done
+text \<open> A local variable lens is defined when its name is in the domain of the store, and the value
+  at that name has the correct type. \<close>
 
-(*
-lemma "lv_lens x \<Longrightarrow> lv_at x n (put\<^bsub>x\<^esub> s v) = lv_at x n s"
-  apply (simp add: lv_at_def)
-  apply auto
-       apply (rotate_tac 2)
-  apply auto
-  apply (simp add: lens_defs)
-*)
+lemma source_lvar_lens: 
+  "\<S>\<^bsub>lvar_lens n :: 'a::injval \<Longrightarrow> _\<^esub> 
+   = {s. n \<in> fdom (get\<^bsub>lstore\<^esub> s) \<and> ffun_app (get\<^bsub>lstore\<^esub> s) n \<in> uvals (utyp TYPE('a::injval))}"
+  by (simp add: lvar_lens_def lens_defined_def comp_mwb_lens source_lens_comp ffun_lens_src source_uval_lens univ_var_def id_lens_def get_ffun_lens)
+
+definition lv_lens :: "('a::injval \<Longrightarrow> 's lvar_scheme) \<Rightarrow> uname \<Rightarrow> bool" where
+"lv_lens x n = (x = lvar_lens n)"
+
+syntax "_lv_lens" :: "id \<Rightarrow> logic" ("lvlens'(_')")
+translations 
+  "lvlens(x)" => "CONST lv_lens x IDLIT(x)"
+  "lvlens(x)" <= "CONST lv_lens x y"
+
+text \<open> For convenience, we allow the notation @{term "lvlens(x)"} to state that the lens bound
+  to identifier @{term x} is a local variable lens with the name @{term "STR ''x''"}. \<close>
+
+lemma mwb_lv_lens [simp]: "lv_lens x n \<Longrightarrow> mwb_lens x"
+  by (simp add: lv_lens_def)
+
+lemma lv_lens_indep_1 [simp]: "\<lbrakk> lv_lens x n; y \<bowtie> lstore \<rbrakk> \<Longrightarrow> x \<bowtie> y"
+  by (metis lens_indep_right_ext lens_indep_sym lv_lens_def lvar_lens_def)
+
+lemma lv_lens_indep_2 [simp]: "\<lbrakk> lv_lens x n; y \<bowtie> lstore \<rbrakk> \<Longrightarrow> y \<bowtie> x"
+  by (meson lens_indep_sym lv_lens_indep_1)
+
+lemma lv_lens_indep_3 [simp]: "\<lbrakk> lv_lens x m; lv_lens y n; m \<noteq> n \<rbrakk> \<Longrightarrow> x \<bowtie> y"
+  by (metis lv_lens_def lvar_lens_indep)
+
+text \<open> The next predicate characterises that a given lens is defined in a particular state. \<close>
+
+definition lvname :: "('a::injval \<Longrightarrow> 's lvar_scheme) \<Rightarrow> uname \<Rightarrow> 's lvar_scheme \<Rightarrow> bool" where 
+[expr_defs]: "lvname x n = (\<guillemotleft>n\<guillemotright> \<in> fdom lstore \<and> lstore(\<guillemotleft>n\<guillemotright>)\<^sub>f \<in> uvals (utyp TYPE('a)))\<^sub>e"
+
+expr_constructor lvname
+
+lemma lv_lens_defined [simp]: "lv_lens x n \<Longrightarrow> \<^bold>D(x) = lvname x n"
+  by (expr_simp add: lv_lens_def source_lvar_lens)
+
+lemma lvname_subst_1 [simp]: "y \<bowtie> lstore \<Longrightarrow> lvname x n ([y \<leadsto> e] s) = lvname x n s"
+  by (simp add: lens_indep.lens_put_irr2 lvname_def subst_id_def subst_upd_def)
+
+lemma lvname_subst_2 [simp]: "\<lbrakk> lv_lens x m; lv_lens y n; m \<noteq> n \<rbrakk> \<Longrightarrow> lvname x m ([y \<leadsto> e] s) = lvname x m s"
+  by (auto simp add: lvname_def subst_upd_def subst_id_def lens_comp_def lv_lens_def lvar_lens_def ffun_lens_def)
+
+lemma lvname_subst_3 [simp]: "\<lbrakk> lv_lens x m; m \<noteq> n \<rbrakk> \<Longrightarrow> lvname x m ([lstore \<leadsto> {\<guillemotleft>n\<guillemotright>} \<Zndres> lstore] s) = lvname x m s"
+  by (auto simp add: lvname_def subst_upd_def subst_id_def lens_comp_def lv_lens_def lvar_lens_def)
+
+syntax "_lvname" :: "id \<Rightarrow> logic" ("LV'(_')")
+translations "LV(x)" => "CONST lvname x IDLIT(x)"
+translations "LV(x)" <= "CONST lvname x y"
+
+text \<open> For convenience, we can use the notation @{term "LV(n)"} to mean that the lens bound to
+  identifier @{term n} is defined in a given state. The syntax translation engine inserts the 
+  string corresponding to the identifier (e.g. @{term "STR ''x''"})
+  \<close>
 
 subsection \<open> Variable Blocks \<close>
 
-definition vblock :: "'v itself \<Rightarrow> (('v::injval \<Longrightarrow> 'a lvar_scheme) \<Rightarrow> ('e, 'a lvar_scheme) htree) \<Rightarrow> ('e, 'a lvar_scheme) htree"
-  where "vblock t B = open_var (utyp TYPE('v)) ;; let_itree (SEXP (\<lambda> s. lvar_lens (length (get\<^bsub>lstack\<^esub> s) - 1))) B ;; close_var"
+text \<open> Extend the variable stack \<close>
+
+definition open_var :: "uname \<Rightarrow> utype \<Rightarrow> ('e, 'a lvar_scheme) htree" where
+"open_var n a = (\<exclamdown>\<guillemotleft>n\<guillemotright> \<notin> fdom lstore! ;; lstore := lstore \<oplus> {\<guillemotleft>n\<guillemotright> \<mapsto> uval_default \<guillemotleft>a\<guillemotright>}\<^sub>f)"
+
+text \<open> Reduce the variable stack \<close>
+
+definition close_var :: "uname \<Rightarrow> ('e, 'a lvar_scheme) htree" where
+"close_var n = (lstore := {\<guillemotleft>n\<guillemotright>} \<Zndres> lstore)"
+
+text \<open> Create a local variable block \<close>
+
+definition vblock :: "uname \<Rightarrow> 'v itself \<Rightarrow> (('v::injval \<Longrightarrow> 'a lvar_scheme) \<Rightarrow> ('e, 'a lvar_scheme) htree) \<Rightarrow> ('e, 'a lvar_scheme) htree"
+  where "vblock n t B = open_var n (utyp TYPE('v))  ;; let_itree (SEXP (\<lambda> s. lvar_lens n)) B ;; close_var n"
 
 syntax "_vblock" :: "id \<Rightarrow> type \<Rightarrow> logic \<Rightarrow> logic" ("var _ :: _./ _" [0, 0, 10] 10)
 
 translations 
-  "_vblock x t e" => "CONST vblock (_TYPE t) (_lvar_abs x t e)"
-  "_vblock x t e" <= "CONST vblock (_TYPE t) (\<lambda> x. e)"
-
-expr_constructor lv_at 
+  "_vblock x t e" => "CONST vblock IDLIT(x) (_TYPE t) (_lvar_abs x t e)"
+  "_vblock x t e" <= "CONST vblock n (_TYPE t) (\<lambda> x. e)"
 
 lemma hl_vblock [hoare_safe]:
   assumes
-    "\<And> x n. lv_lens x n \<Longrightarrow> H{length lstack = \<guillemotleft>n\<guillemotright> + 1 \<and> P\<lbrakk>butlast lstack/lstack\<rbrakk>} B x {Q\<lbrakk>butlast lstack/lstack\<rbrakk>}"
-  shows "H{P} var x :: 't::injval. B x {Q}"
-proof -
-  have a: "\<And> x n. H{length lstack = \<guillemotleft>n\<guillemotright> + 1 \<and> P\<lbrakk>butlast lstack/lstack\<rbrakk> \<and> \<guillemotleft>lv_lens x n\<guillemotright>} B x {Q\<lbrakk>butlast lstack/lstack\<rbrakk>}"
-    using assms hoare_rel_triple_def by force 
-
-  thus ?thesis
-    apply (simp add: vblock_def open_var_def close_var_def)
-    apply (rule hoare_safe)
-      apply simp
-     apply (rule hoare_safe)
-     apply (rule hoare_safe)
-     apply (rule hl_conseq)
-    apply (rule a)
-    apply (simp add: lv_at_def)
-  using assms(1)
-   apply (simp add: lv_at_def lvar_lens_def lv_lens_def expr_defs univ_var_def id_lens_def)
+    "\<And> x. lv_lens x n \<Longrightarrow> H{lvname x n \<and> P\<lbrakk>{\<guillemotleft>n\<guillemotright>} \<Zndres> lstore/lstore\<rbrakk>} B x {Q\<lbrakk>{\<guillemotleft>n\<guillemotright>} \<Zndres> lstore/lstore\<rbrakk>}"
+  shows "H{P} vblock n TYPE('t::injval) (\<lambda> x. B x) {Q}"
+  apply (simp add: vblock_def open_var_def close_var_def kcomp_assoc)
+  apply (rule hoare_safe)
+  apply (rule hoare_safe)
+    apply simp
+   apply (rule hoare_safe)
+   apply (rule hoare_safe)
+   apply (rule hl_conseq)
+     apply (rule assms(1))
+     apply (simp add: lv_lens_def)
+    apply (simp add: lv_lens_def lvname_def uvals_def)
     apply expr_auto
-  using assms(1)
+    apply (metis (no_types, lifting) Diff_disjoint Diff_insert_absorb fdom_fdom_res fdom_plus fdom_res_fdom fdom_res_twice ffun_split_domain sup_bot_left)
    apply expr_simp
   apply auto[1]
   done
-qed
-
-(*
-lemma hl_vblock [hoare_safe]:
-  assumes
-    "`P \<longrightarrow> \<guillemotleft>n\<guillemotright> = length lstack`"
-    "\<And> x. lv_lens x n \<Longrightarrow> H{length lstack = \<guillemotleft>n\<guillemotright> + 1 \<and> P\<lbrakk>butlast lstack/lstack\<rbrakk>} B x {Q\<lbrakk>butlast lstack/lstack\<rbrakk>}"
-  shows "H{P} var x :: 't::injval. B x {Q}"
-proof -
-  have a: "\<And> x. H{length lstack = \<guillemotleft>n\<guillemotright> + 1 \<and> P\<lbrakk>butlast lstack/lstack\<rbrakk> \<and> \<guillemotleft>lv_lens x n\<guillemotright>} B x {Q\<lbrakk>butlast lstack/lstack\<rbrakk>}"
-    using assms(2) hoare_rel_triple_def by force 
-
-  thus ?thesis
-    apply (simp add: vblock_def open_var_def close_var_def)
-    apply (rule hoare_safe)
-      apply simp
-     apply (rule hoare_safe)
-     apply (rule hoare_safe)
-     apply (rule hl_conseq)
-    apply (rule a)
-    apply (simp add: lv_at_def)
-  using assms(1)
-   apply (simp add: lv_at_def lvar_lens_def lv_lens_def expr_defs univ_var_def id_lens_def)
-    apply expr_auto
-  using assms(1)
-   apply expr_simp
-  apply auto[1]
-  done
-qed
-*)
-
-lemma "H{length lstack = \<guillemotleft>k\<guillemotright>} var x :: nat. var y :: int. Skip {True}"
-  apply (rule hl_vblock)
-  apply (subst_eval)
-  apply (rule hl_vblock)
-  apply (subst_eval)
-  oops
-  
 
 end
